examples/rel/WhileReify.fst
@@ -52,15 +52,13 @@ type com =
 | While  : cond:exp -> body:com -> variant:variant -> com
 
 
-reifiable val interpret_exp_st : e:exp -> ST int
+reifiable val interpret_exp_st : e:exp -> IS int
   (requires (fun _ -> True))
   (ensures  (fun h r h' -> h == h'))
 reifiable let rec interpret_exp_st e =
   match e with
   | AInt i -> i
-  | AVar x -> let h = STATE?.get() in
-              assume(h `contains_a_well_typed` x); (* XXX: now needing this *)
-              !x
+  | AVar x -> read x
   | AOp o e1 e2 ->
     let a = interpret_exp_st e1 in
     let b = interpret_exp_st e2 in
@@ -79,29 +77,32 @@ let decr_while h c =
 
 exception OutOfFuel
 
-reifiable val interpret_com_st : c:com -> h0:heap -> ST unit
+reifiable val interpret_com_st : c:com -> h0:heap -> IS unit
   (requires (fun h -> h == h0))
   (ensures (fun _ _ _ -> True))
   (decreases %[c; decr_while h0 c])
 reifiable let rec interpret_com_st c h0 =
   match c with
   | Skip -> ()
-  | Assign x e -> let h = STATE?.get() in
-                  assume(h `contains_a_well_typed` x); (* XXX: now needing this *)
-                  x := interpret_exp_st e
+  | Assign x e ->
+    let v = interpret_exp_st e in
+    write x v
   | Seq c1 c2 ->
     begin
-      interpret_com_st c1 (STATE?.get());
-      interpret_com_st c2 (STATE?.get())
+      let h1 = (INT_STORE?.get()) in
+      interpret_com_st c1 h1;
+      let h2 = (INT_STORE?.get()) in
+      interpret_com_st c2 h2
     end
   | If e ct cf ->
       let c = if interpret_exp_st e = 0 then cf else ct in
-      interpret_com_st c (STATE?.get())
+      let h = (INT_STORE?.get()) in
+      interpret_com_st c h
   | While e body v ->
     if interpret_exp_st e <> 0 then
       begin
       (*   let m0 = interpret_exp_st v in *)
-      (*   interpret_com_st body (STATE?.get()); *)
+      (*   interpret_com_st body (INT_STORE?.get()); *)
       (*   let m1 = interpret_exp_st v in *)
       (* proving recursive terminating relies of interpret_exp not
          changing the state? somehow F* can't prove this although
@@ -109,12 +110,13 @@ reifiable let rec interpret_com_st c h0 =
       (* working around by using reify *)
         let m0, _ = reify (interpret_exp_st v) h0 in
         interpret_com_st body h0;
-        let h1 = STATE?.get() in
+        let h1 = INT_STORE?.get() in
         let m1, _ = reify (interpret_exp_st v) h1 in
         if m0 > m1 && m1 >= 0 then
-          interpret_com_st c (STATE?.get())
+          let h2 = (INT_STORE?.get()) in
+          interpret_com_st c h2
         else
-          () (* raise OutOfFuel -- XXX: no exceptions yet *)
+          raise_ () (* raise OutOfFuel -- XXX: no exceptions yet *)
       end
 
 let interpret_com h c = normalize_term (reify (interpret_com_st c h) h)
